\lecture{11}{2021-11-23}{}

\begin{prob}{Putnam 2011, A3}{}
        Find a real number $c$ and a positive number $L$ for which
        \[\lim_{r\to\infty}\frac{r^c\int_0^{\pi/2}x^r\sin x\,dx}{\int_0^{\pi/2}x^r\cos x\,dx}=L.\]
\end{prob}

\begin{sol}{}{}
	The answer is \(c = -1\) and \(L = 2/\pi\).
	Taylor series implies that 
	\begin{align*}
		\sin x  &= \sum_{i=0}^\infty \frac{(-1)^i}{(2i+1)!} x^{2i+1} \\
		\cos x  &= \sum_{i=0}^\infty \frac{(-1)^i}{(2i)!} x^{2i}
	\end{align*}

	Then, we have 
	\begin{align*}
		&\lim_{r\to \infty}
		{r(\pi/2)^{-r-1} \int_0^{\pi/2} x^r \sin x\,dx} \\
		=& \lim_{r\to \infty}
		{\int_0^{\pi/2} \sum_{i=0}^\infty r(\pi/2)^{-r-1}\frac{(-1)^i}{(2i+1)!} x^{2i+1+r}\,dx} \\
		=& \lim_{r\to \infty}
		{\sum_{i=0}^\infty \int_0^{\pi/2} r(\pi/2)^{-r-1}\frac{(-1)^i}{(2i+1)!} x^{2i+1+r}\,dx} \\
		=& \lim_{r\to \infty}
		{\sum_{i=0}^\infty r(\pi/2)^{-r-1}\frac{(-1)^i}{(2i+2+r)(2i+1)!} \left(\pi/2\right)^{2i+2+r}} \\
		=& \lim_{r\to \infty}
		{\sum_{i=0}^\infty \frac{r}{2i+2+r}\frac{(-1)^i}{(2i+1)!} \left(\pi/2\right)^{2i+1}} \\
		=& \sum_{i=0}^\infty \lim_{r\to \infty}
		{\frac{r}{2i+2+r}\frac{(-1)^i}{(2i+1)!} \left(\pi/2\right)^{2i+1}} \\
		=& \sum_{i=0}^\infty
		{\frac{(-1)^i}{(2i+1)!} \left(\pi/2\right)^{2i+1}} \\
		=& \sum_{i=0}^\infty
		{\frac{(-1)^i}{(2i+1)!} \left(\pi/2\right)^{2i+1}} \\
		=& \sin\left(\pi/2\right) = 1
	\end{align*}

	And we also have
	\begin{align*}
		&\lim_{r\to \infty}
		r^2(\pi/2)^{-r-1} \int_0^{\pi/2} x^r \cos x\,dx\\
		=& \lim_{r\to \infty}
		\int_0^{\pi/2} \sum_{i=0}^\infty r^2(\pi/2)^{-r-1} \frac{(-1)^i}{(2i)!} x^{2i}\,dx \\
		=& \lim_{r\to \infty}
		\sum_{i=0}^\infty \int_0^{\pi/2} r^2(\pi/2)^{-r-1} \frac{(-1)^i}{(2i)!} x^{2i}\,dx \\
		=& \lim_{r\to \infty}
		\sum_{i=0}^\infty \frac{r^2}{2i+1+r}\frac{(-1)^i}{(2i)!} (\pi/2)^{2i} \\
		=& \lim_{r\to \infty} \left(
			\frac{r^2}{r+1} + \sum_{i=1}^\infty \frac{r^2}{2i+1+r}\frac{(-1)^i}{(2i)!} (\pi/2)^{2i}
		\right) \\
		=& \lim_{r\to \infty} \left(
			\frac{r^2}{r+1} + \sum_{i=1}^\infty \frac{r^2}{(2i+1+r)(2i)}\frac{(-1)^i}{(2i-1)!} (\pi/2)^{2i}
		\right) \\
		=& \lim_{r\to \infty} \left(
			\frac{r^2}{r+1} + \sum_{i=1}^\infty \frac{r}{r+1}\left(\frac{r}{2i} - \frac{r}{2i+1+r}\right)\frac{(-1)^i}{(2i-1)!} (\pi/2)^{2i}
		\right) \\
		=& \lim_{r\to \infty} \left(
			\left(\sum_{i=0}^\infty \frac{r^2}{r+1}\frac{(-1)^i}{(2i)!} (\pi/2)^{2i}\right) - 
			\left(\sum_{i=1}^\infty \frac{r^2}{(r+1)(2i+1+r)}\frac{(-1)^i}{(2i-1)!} (\pi/2)^{2i}\right)
		\right) \\
		=& \lim_{r\to \infty} \left(
			\frac{r^2}{r+1}\left(\sum_{i=0}^\infty \frac{(-1)^i}{(2i)!} (\pi/2)^{2i}\right) - 
			\left(\sum_{i=1}^\infty \frac{r^2}{(r+1)(2i+1+r)}\frac{(-1)^i}{(2i-1)!} (\pi/2)^{2i}\right)
		\right) \\
		=& \lim_{r\to \infty} \left(
			\frac{r^2}{r+1}\cos(\pi/2) - 
			\left(\sum_{i=1}^\infty \frac{r^2}{(r+1)(2i+1+r)}\frac{(-1)^i}{(2i-1)!} (\pi/2)^{2i}\right) 
		\right) \\
		=& \lim_{r\to \infty}
		\sum_{i=1}^\infty \frac{r^2}{(r+1)(2i+1+r)}\frac{(-1)^{i+1}}{(2i-1)!} (\pi/2)^{2i} \\
		=& \sum_{i=1}^\infty \lim_{r\to \infty} \frac{r^2}{(r+1)(2i+1+r)}\frac{(-1)^{i+1}}{(2i-1)!} (\pi/2)^{2i} \\
		=& \sum_{i=1}^\infty \frac{(-1)^{i+1}}{(2i-1)!} (\pi/2)^{2i} \\
		=& \sum_{i=0}^\infty \frac{(-1)^{i}}{(2i+1)!} (\pi/2)^{2i+2} \\
		=& (\pi/2) \sum_{i=0}^\infty \frac{(-1)^{i}}{(2i+1)!} (\pi/2)^{2i+1} \\
		=& (\pi/2)\sin(\pi/2) = \pi/2.
	\end{align*}

	Finally, this implies that
	\begin{align*}
		\lim_{r\to \infty}
		\frac%
		{r^{-1} \int_0^{\pi/2} x^r \sin x\,dx}%
		{\int_0^{\pi/2} x^r \cos x\,dx}
		&=
		\lim_{r\to \infty}
		\frac%
		{r  (\pi/2)^{-r-1} \int_0^{\pi/2} x^r \sin x\,dx}%
		{r^2(\pi/2)^{-r-1} \int_0^{\pi/2} x^r \cos x\,dx}\\
		&=
		\frac%
		{\lim_{r\to \infty}r  (\pi/2)^{-r-1} \int_0^{\pi/2} x^r \sin x\,dx}%
		{\lim_{r\to \infty}r^2(\pi/2)^{-r-1} \int_0^{\pi/2} x^r \cos x\,dx}
		= \frac{2}{\pi}
	\end{align*}
\end{sol}
