\lecture{8}{2021-11-03}{}

\begin{prob}{}{}
	Find the $2000$\textsuperscript{th} digit in the square root of $N = 11\dots1$, where $N$ contains $1998$ digits, all of them $1$'s.
\end{prob}

\begin{sol}{}{}
	The answer is \boxed{6.}
	We can estimate \[
		\sqrt{\frac{10^{1998} - 1}{9}} \approx \sqrt{\frac{10^{1998}}{9}} = \frac{10^{999}}{3}.
	\]
	How good is this estimate?
	\begin{align*}
		\left(\frac{10^{999}}{3} - \sqrt{\frac{10^{1998} - 1}{9}}\right)
		\left(\frac{10^{999}}{3} + \sqrt{\frac{10^{1998} - 1}{9}}\right) &=
		\frac{10^{1998}}{9} - \frac{10^{1998}-1}{9} \\
		&= \frac{1}{9},
	\end{align*}
	thus, by using the estimative $\sqrt{\frac{10^{1998} - 1}{9}} \approx \frac{10^{999}}{3}$,
	\begin{align*}
		\frac{10^{999}}{3} - \sqrt{\frac{10^{1998} - 1}{9}} \approx \frac{1}{6 \cdot 10^{999}},
	\end{align*}
	which sadly implies that our estimative is not good enough to evaluate the \(2000\)\textsuperscript{th}. However, now we have a new estimative:
	\[
		\sqrt{\frac{10^{1998} - 1}{9}} \approx \frac{10^{999}}{3} - \frac{1}{6 \cdot 10^{999}}.
	\]
	Again, how good is this estimative?
	\begin{align*}
		\left(\sqrt{\tfrac{10^{1998} - 1}{9}} - \left(\tfrac{10^{999}}{3} - \tfrac{1}{6 \cdot 10^{999}}\right)\right)
		\left(\sqrt{\tfrac{10^{1998} - 1}{9}} + \left(\tfrac{10^{999}}{3} - \tfrac{1}{6 \cdot 10^{999}}\right)\right)
		&= 
		\tfrac{10^{1998} - 1}{9} - \left(\tfrac{10^{999}}{3} - \tfrac{1}{6 \cdot 10^{999}}\right)^2 \\
		&= \tfrac{1}{36 \cdot 10^{1998}},
	\end{align*}
	so we know that \[
		\sqrt{\tfrac{10^{1998} - 1}{9}} - \left(\tfrac{10^{999}}{3} - \tfrac{1}{6 \cdot 10^{999}}\right) < \frac{1}{10^{1010}},
	\]
	which is good enough to imply that the \(2000\)\textsuperscript{th} digit of \(\sqrt{\tfrac{10^{1998} - 1}{9}}\) is equal to the \(2000\)\textsuperscript{th} digit of \(\tfrac{10^{999}}{3} - \tfrac{1}{6 \cdot 10^{999}}\), which is \(6\).
\end{sol}

\begin{prob}{Putnam 2014, A3}{}
	Let $a_0=5/2$ and $a_k=a_{k-1}^2-2$ for $k\ge 1.$ Compute \[\prod_{k=0}^{\infty}\left(1-\frac1{a_k}\right)\] in closed form.
\end{prob}

\begin{sk}{}{}
	\textcolor{red}{The full solution is to be done.} The answer is \(\boxed{3/7.}\) Prove by induction that \[
		a_n = 2^{2^n} + 2^{-2^n}.
	\]
	Then, the product we want to evaluate is \[
		\prod_{k=0}^\infty \frac{(1/4)^{2^k} - (1/2)^{2^k} + 1}{(1/4)^{2^k} + 1} = 
		\prod_{k=0}^\infty \frac{(1/8)^{2^k} + 1}{((1/4)^{2^k} + 1)((1/2)^{2^k} + 1)}.
	\]
	It suffices to show that \[
		\prod_{k=0}^\infty x^{2^k} + 1 = \frac{1}{1 - x},
	\] and plug the results for \(x = 1/2\), \(x = 1/4\), and \(x = 1/8\).

	Finally, the answer is \[
		\frac{8/7}{(2/1)(4/3)} = \frac{3}{7}.
	\]
\end{sk}
